doc-src/TutorialI/Types/Overloading.thy
@@ -16,12 +16,4 @@ prefix_def:
   "xs <<= (ys::'a::ordrel list)  \<equiv>  \<exists>zs. ys = xs@zs"
 strict_prefix_def:
   "xs << (ys::'a::ordrel list)   \<equiv>  xs <<= ys \<and> xs \<noteq> ys"
-  
-text{*
-We could also have made the second definition non-overloaded once and for
-all: @{prop"x << y \<equiv> x <<= y \<and> x \<noteq> y"}.  This would have saved us writing
-many similar definitions at different types, but it would also have fixed
-that @{text <<} is defined in terms of @{text <<=} and never the other way
-around. Below you will see why we want to avoid this asymmetry.
-*}
 (*<*)end(*>*)
